Update dec_list proof, add main program

programs.v
@@ -2,18 +2,34 @@ From pv Require Import language.
 From pv Require Import proofmode.
 Import language_notation hoare_notation.
 
+Fixpoint alloc_list (l : list nat) : val :=
+  closure: "_" =>
+    match l with
+    | [] => NONE
+    | n :: l' =>
+        let: "l'" := alloc_list l' () in
+        let: "l" := alloc (n, "l'") in
+        SOME "l"
+    end.
+
 Definition dec_list : val :=
   recclosure: "dec_list" "l" =>
     match: "l" with
-    | NONE => VUnit
+    | NONE => ()
     | SOME "p" =>
-        let: "x" := EFst !"p" in
-        let: "l" := ESnd !"p" in
+        let: "x" := fst !"p" in
+        let: "l" := snd !"p" in
         if: "x" =: 0
-          then EThrow tt ()
+          then throw tt ()
           else "p" <- ("x" -: 1, "l");;
                "dec_list" "l"
     end.
+
+Definition main (l : list nat) : val :=
+  closure: "_" =>
+    let: "l" := alloc_list l () in
+    (dec_list "l";; "l")
+      catch: tt "_" => "l".
 
 Fixpoint is_list (l : list nat) (v : val) : sepProp :=
   match l with
@@ -24,13 +40,34 @@ Fixpoint is_list (l : list nat) (v : val) : sepProp :=
       is_list l' v'
   end.
 
+Lemma alloc_list_spec l :
+  {{ EMP }}
+    alloc_list l ()
+  {{ v, is_list l v }}
+  {{ _ _, FALSE }}.
+Proof.
+  iIntros "_".
+  iInduction l as [| n l'] "IH"; simpl; iApply App_wp.
+  - by iApply InjL_wp.
+  - iApply Let_wp. iApply "IH"; iSplit.
+    + iIntros (v') "Hv'". iApply Let_wp.
+      iApply Pair_wp. iApply Alloc_wp; iIntros (p) "Hp".
+      iApply InjR_wp. eauto with iFrame.
+    + by iIntros (??) "?".
+Qed.
+
+Local Notation positive := (fun x => x ≠ 0).
+
 Lemma dec_list_spec l v :
   {{ is_list l v }}
     dec_list v
-  {{ vret, @[ vret = () ] ** is_list (map pred l) v }}
-  {{ t vex, @[ t = tt /\ vex = () ] **
-            Ex l1 l2, @[ l = l1 ++ l2 ] **
-                      is_list (map pred l1 ++ l2) v }}.
+  {{ vret, @[ vret = () ] **
+           @[ Forall positive l ] **
+           is_list (map pred l) v }}
+  {{ t vex, @[ t = tt ] ** @[ vex = () ] **
+            Ex l1 l2, @[ l = l1 ++ 0 :: l2 ] **
+                      @[ Forall positive l1 ] **
+                      is_list (map pred l1 ++ 0 :: l2) v }}.
 Proof.
   iIntros "Hv".
   iInduction l as [| n l'] "IH" forall (v); simpl; iApply AppRec_wp.
@@ -40,16 +77,50 @@ Proof.
     iApply Let_wp. iApply Load_wp; iIntros "{$Hp} Hp". iApply Fst_wp.
     iApply Let_wp. iApply Load_wp; iIntros "{$Hp} Hp". iApply Snd_wp.
     iApply Op_wp. destruct (n =? 0) eqn: Hn.
-    + iApply If_true_wp. iApply Throw_Val_wp. iSplit; [done |].
-      iExists [], (n :: l'); simpl; eauto 6 with iFrame.
-    + iApply If_false_wp. iApply Seq_wp.
+    + apply beq_nat_true in Hn as ->.
+      iApply If_true_wp. iApply Throw_Val_wp. do 2 (iSplit; [done |]).
+      iExists [], l'; simpl; eauto 6 with iFrame.
+    + apply beq_nat_false in Hn.
+      iApply If_false_wp. iApply Seq_wp.
       iApply Op_wp. iApply Pair_wp. iApply Store_wp; iIntros "{$Hp} Hp".
       iApply ("IH" with "Hv'"); iSplit.
-      * iIntros (v) "[% Hv']".
+      * iIntros (vret) "(% & %Hl' & Hv')".
         replace (pred n) with (n - 1) by lia.
-        eauto with iFrame.
-      * iIntros (t v) "(% & %l1 & %l2 & -> & Hv')". iSplit; [done |].
+        eauto 8 with iFrame.
+      * iIntros (t vex) "(% & % & %l1 & %l2 & -> & %Hl1 & Hv')";
+          do 2 (iSplit; [done |]).
         iExists (n :: l1), l2; simpl.
         replace (pred n) with (n - 1) by lia.
-        eauto 6 with iFrame.
+        eauto 8 with iFrame.
+Qed.
+
+Lemma main_spec l :
+  {{ EMP }}
+    main l ()
+  {{ v, @[ Forall positive l ] ** is_list (map pred l) v \//
+        Ex l1 l2, @[ l = l1 ++ 0 :: l2 ] **
+          is_list (map pred l1 ++ 0 :: l2) v }}
+  {{ _ _, FALSE }}.
+Proof.
+  iIntros "_". iApply App_wp. iApply Let_wp.
+  iApply (alloc_list_spec with "[//]"); iSplit.
+  - iIntros (v) "Hv". iApply Catch_wp. iApply Seq_wp.
+    iApply (dec_list_spec with "Hv"); iSplit.
+    + iIntros (?) "(% & %Hl & Hv)". iApply Val_wp. eauto with iFrame.
+    + iIntros (t ?) "(-> & % & %l1 & %l2 & -> & %Hl1 & Hv)".
+      rewrite tag_dec_eq. iApply Let_Val_wp. iApply Val_wp. eauto with iFrame.
+  - by iIntros (??) "?".
+Qed.
+
+Lemma main_spec' l :
+  {{ @[ Forall positive l ] }}
+    main l ()
+  {{ v, is_list (map pred l) v }}
+  {{ _ _, FALSE }}.
+Proof.
+  iStartProof; iIntros (Hl).
+  iApply (main_spec with "[//]"); iSplit.
+  - iIntros (v) "[[_ Hv] | (%l1 & %l2 & -> & ?)]"; [done |].
+    apply Forall_app in Hl as [Hl1 Hl2]. by inv Hl2.
+  - by iIntros (??) "?".
 Qed.
